HMAC_spec_concat.v
@@ -128,6 +128,69 @@ Proof.
   * apply block_8. apply len.
 Qed. 
 
+Lemma NPeano_divide_trans a b c: NPeano.divide a b -> 
+      NPeano.divide b c -> NPeano.divide a c.
+Proof. intros. destruct H; destruct H0. subst.
+  exists (x0 * x)%nat. apply mult_assoc.
+Qed. 
+(*
+Lemma R_hash_blocks_bits_length: forall f r msg
+      (HR: forall (z:Blist), z<> nil -> NPeano.divide (length r) (length (f r (firstn 512 z))))
+      h (Hh: R_hash_blocks_bits f r msg h) ,
+      NPeano.divide (length r) (length h).
+Proof. intros.
+SearchAbout R_hash_blocks_bits.
+  eapply (R_hash_blocks_bits_rec). Focus 3. eassumption.
+  intros. exists 1%nat. omega.
+  intros. subst. eapply NPeano_divide_trans. 2: eassumption. clear H.
+ destruct _x. contradiction. clear y.
+  SearchAbout NPeano.divide. simpl in *.  intros y.
+  induction y.
+  intros. unfold hash_blocks_bits. simpl. exists 1%nat. omega.
+  intros. unfold hash_blocks_bits. 
+    remember (hash_blocks_bits_terminate f x (a :: y)%list).
+    destruct s as [v [p Hvp]]. clear Heqs.
+    unfold hash_blocks_bits_F in Hvp. simpl in Hvp. fold hash_blocks_bits_F in Hvp.  unfold NPeano.divide. SearchAbout NPeano.divide. simpl. Z.divide.
+Admitted.
+Lemma hash_blocks_bits_length: forall f r msg
+      (HR: forall (z:Blist), z<> nil -> NPeano.divide (length r) (length (f r (firstn 512 z)))),
+      NPeano.divide (length r) (length (hash_blocks_bits f r msg)).
+Proof.
+Print R_hash_blocks_bits.
+  Check (hash_blocks_bits_rect f).
+  intros. exists 1%nat. omega.
+  intros. subst. eapply NPeano_divide_trans. 2: eassumption. clear H.
+ destruct _x. contradiction. clear y.
+  SearchAbout NPeano.divide. simpl in *.  intros y.
+  induction y.
+  intros. unfold hash_blocks_bits. simpl. exists 1%nat. omega.
+  intros. unfold hash_blocks_bits. 
+    remember (hash_blocks_bits_terminate f x (a :: y)%list).
+    destruct s as [v [p Hvp]]. clear Heqs.
+    unfold hash_blocks_bits_F in Hvp. simpl in Hvp. fold hash_blocks_bits_F in Hvp.  unfold NPeano.divide. SearchAbout NPeano.divide. simpl. Z.divide.
+Admitted.
+(*
+Lemma hash_blocks_bits_terminate_length: forall f x y,
+      NPeano.divide (length x) (fst (hash_blocks_bits_terminate f x y)).
+       (a,_) => NPeano.divide (length x) (length a)
+      end.*)
+SearchAbout hash_blocks_bits.
+Lemma HBBF_length hash_block_bit: forall msg r,
+      NPeano.divide (length r) (length (hash_blocks_bits_F r msg)). (*
+Lemma hash_blocks_bits_terminate_length f x y: 
+      match hash_blocks_bits_terminate f x y with
+       (a,b) => length a = 8%nat
+      end.*)
+Lemma hash_blocks_bits_length f: forall y x, NPeano.divide (length x) (length (hash_blocks_bits f x y)).
+Proof. hash_blocks_bits_rect intros y.
+  induction y.
+  intros. unfold hash_blocks_bits. simpl. exists 1%nat. omega.
+  intros. unfold hash_blocks_bits. 
+    remember (hash_blocks_bits_terminate f x (a :: y)%list).
+    destruct s as [v [p Hvp]]. clear Heqs.
+    unfold hash_blocks_bits_F in Hvp. simpl in Hvp. fold hash_blocks_bits_F in Hvp.  unfold NPeano.divide. SearchAbout NPeano.divide. simpl. Z.divide.
+Admitted.
+*)
 Theorem HMAC_concat_pad : forall (k m : Blist) (op ip : Blist),
                             length k = b ->
                             length ip = b ->
@@ -151,14 +214,17 @@ Proof.
   f_equal.
 
   rewrite <- splitandpad_eq.
-  Check fpad_eq.
   rewrite <- fpad_eq.           (* wants the InBlocks 8 *)
   reflexivity.
 
   * apply BLxor_length. apply len_k. apply len_op.
   *
     unfold HMAC_Concat.h_star.
-    Print intsToBits.
+    Print intsToBits. SearchAbout InBlocks.
+(* Lennart: here's a minor attemp to psuh this further:
+     rewrite -> hash_blocks_bits_equation.
+    unfold sha_h.
+    apply InBlocks_len. This goal here triggered the attempt to prove the divide-slemmas above*)
     rewrite -> hash_blocks_bits_equation.
     unfold sha_h.
     Check common_lemmas.length_hash_block.
